$T_(p q)$ transforms the pair $(a,b)$ such that
$a <- b q + a q + a p "and" b <- b p + a q$. #linebreak()
After two transformations we get: #linebreak()
$a  
<-& (b p + a q)q + (b q + a q + a p)q +
(b q + a q + a p)p \
=& p q b + q^2 a + q^2 b + q^2 a + p q a + p q b + p q a + p^2 a \
=& p^2 a + 2p q a + 2p q b + 2q^2 a + q^2 b \
=& a(p^2 + 2p q + 2q^2) + b(2p q + q^2) 
#linebreak()
b 
<-& (b p + a q)p + (b q + a q + a p)q \
=& p^2 b + p q a + q^2 b + q^2 a + p q a \
=& p^2 b + 2p q a + q^2 a + q^2 b \
=& b(p^2 + q^2) + a(2 p q + q^2). #linebreak()
"From above,"
a 
<-& a(p^2 + 2p q + 2q^2) + b(2p q + q^2) \
=& b(2p q + q^2) + a(2p q + q^2) + a(p^2 + q^2).$ #linebreak()
Therefore, if we let $p' = p^2 + q^2$ and $q' = 2p q + q^2$,
then we can represent applying $T_(p q)$ twice with the single
transformation $T_(p' q')$.


